proof/correctness/avx2/Kyber_AVX2_cf.ec
@@ -1,6 +1,7 @@
 require import AllCore List Int IntDiv CoreMap Real Number LoopTransform.
 from Jasmin require import JWord.
-require import Array32 Array64 Array128 Array168 Array256 Array384.
+require import Array16 Array32 Array64 Array128 Array168 Array256 Array384.
+require import Jkem.
 require import Kyber.
 
 (* TODO: prove equivalence w/ EncDec using LoopTransform
@@ -16,14 +17,17 @@ n.b: check libjc/proof/crypto_stream/chacha20/ChaCha20_pavx2_cf.ec
 *)
 
 module EncDec_AVX2 = {
-   proc body_decode4(t: W8.t Array128.t * ipoly, i: int): ipoly = {
-     var r, a;
-     (a, r) <- t;
-
-     (* r.[8*i+2*j+0]  <- to_uint a.[8*i+j] %% 16; *)
-     (* r.[8*i+2*j+1]  <- to_uint a.[8*i+j] %/ 16; *)
-
-     return r;
+   proc decode12(a : W8.t Array384.t) : ipoly = {
+       var i;
+       var r : ipoly;
+       r <- witness;
+       i <- 0;
+       while (i < 128) {
+          r.[i*2+0]  <- to_uint a.[3*i] + to_uint a.[3*i+1] %% 2^4 * 2^8;
+          r.[i*2+1]  <- to_uint a.[3*i+2] * 2^4 + to_uint a.[3*i+1] %/ 2^4;
+          i <- i + 1;
+       }
+       return r;
    }
 
    proc decode4(a : W8.t Array128.t) : ipoly = {
@@ -42,6 +46,63 @@ module EncDec_AVX2 = {
        }
        return r;
    }
+
+  proc decode1(a : W8.t Array32.t) : ipoly = {
+    var i,j;
+    var r : ipoly;
+    r <- witness;
+    i <- 0;
+    while (i < 4) {
+      j <- 0;
+      while(j < 4) {
+        r <- Array256.fill (fun k => b2i a.[k %/ 8].[k %% 8]) (32*i + j*8) 8 r;
+        j <- j + 1;
+      }
+
+      j <- 0;
+      while(j < 4) {
+        r <- Array256.fill (fun k => b2i a.[k %/ 8].[k %% 8]) (128 + 32*i + j*8) 8 r;
+        j <- j + 1;
+      }
+      (* TODO: prove equivalence ??
+      while(j < 8){
+        r.[64*i+j*8+0] <- b2i a.[8*i+j].[0];
+        r.[64*i+j*8+1] <- b2i a.[8*i+j].[1];
+        r.[64*i+j*8+2] <- b2i a.[8*i+j].[2];
+        r.[64*i+j*8+3] <- b2i a.[8*i+j].[3];
+        r.[64*i+j*8+4] <- b2i a.[8*i+j].[4];
+        r.[64*i+j*8+5] <- b2i a.[8*i+j].[5];
+        r.[64*i+j*8+6] <- b2i a.[8*i+j].[6];
+        r.[64*i+j*8+7] <- b2i a.[8*i+j].[7];
+      }
+      *)
+      i<-i+1;
+    }
+
+    return r;
+  }
+
+  proc encode12(a : ipoly) : W8.t Array384.t = {
+     var fi1,fi2,i,k;
+     var r : W8.t Array384.t;
+
+     i <- 0;
+     while (i < 2) {
+       k <- 0;
+
+       while(k < 64) {
+         fi1 <- a.[128*i + k];
+         fi2 <- a.[128*i + k + 1];
+         r.[192*i+3*k] <- W8.of_int fi1;
+         r.[192*i+3*k+1] <- W8.of_int ((fi2 %% 2^4) * 2^4 + fi1 %/ 2^8);
+         r.[192*i+3*k+2] <- W8.of_int (fi2 %/ 2^4);
+         k <- k + 2;
+       }
+
+       i <- i + 1;
+     }
+     return r;
+  }
 
    proc encode4(p : ipoly) : W8.t Array128.t = {
        var fi,fi1,i,k;
@@ -85,38 +146,37 @@ module EncDec_AVX2 = {
     return ra;      
   }
 
-  proc decode1(a : W8.t Array32.t) : ipoly = {
-    var i,j;
-    var r : ipoly;
-    r <- witness;
-    i <- 0;
-    while (i < 4) {
-      j <- 0;
-      while(j < 4) {
-        r <- Array256.fill (fun k => b2i a.[k %/ 8].[k %% 8]) (32*i + j*8) 8 r;
-        j <- j + 1;
-      }
 
-      j <- 0;
-      while(j < 4) {
-        r <- Array256.fill (fun k => b2i a.[k %/ 8].[k %% 8]) (128 + 32*i + j*8) 8 r;
-        j <- j + 1;
-      }
-      (* TODO: prove equivalence ??
-      while(j < 8){
-        r.[64*i+j*8+0] <- b2i a.[8*i+j].[0];
-        r.[64*i+j*8+1] <- b2i a.[8*i+j].[1];
-        r.[64*i+j*8+2] <- b2i a.[8*i+j].[2];
-        r.[64*i+j*8+3] <- b2i a.[8*i+j].[3];
-        r.[64*i+j*8+4] <- b2i a.[8*i+j].[4];
-        r.[64*i+j*8+5] <- b2i a.[8*i+j].[5];
-        r.[64*i+j*8+6] <- b2i a.[8*i+j].[6];
-        r.[64*i+j*8+7] <- b2i a.[8*i+j].[7];
-      }
-      *)
-      i<-i+1;
+
+}.
+
+module Kyber_AVX2_cf = {
+  proc __fqmul_x16 (a b: W16.t Array16.t) : W16.t Array16.t = {
+    var i;
+    var t: W16.t;
+    var rd:W16.t Array16.t;
+
+    i <- 0;
+    while(i < 16) {
+      t <@ M.__fqmul(a.[i], b.[i]);
+      rd.[i] <- t;
+      i <- i + 1;
     }
 
-    return r;
+    return (rd);
+  }
+
+  proc __red_x16 (r: W16.t Array16.t) : W16.t Array16.t = {
+    var i;
+    var t: W16.t;
+
+    i <- 0;
+    while(i < 16) {
+      t <@ M.__barrett_reduce(r.[i]);
+      r.[i] <- t;
+      i <- i + 1;
+    }
+
+    return (r);
   }
 }.
